Tutorial: three xor-based examples (#651)

demos/tutorial.v
@@ -24,9 +24,12 @@ Tutorial
 ========
 
 Welcome! This is a quick primer for designing circuits with Cava. We'll walk
-through a few small examples end-to-end. This tutorial assumes some familiarity
-with Coq syntax. Use Ctrl+down and Ctrl+up to step through the Coq code along
-with the tutorial.
+through a few small examples end-to-end. This tutorial will not explain Coq
+syntax in depth, but will use the same few patterns throughout; you shouldn't
+need to know Coq to follow along.
+
+Use Ctrl+down and Ctrl+up to step through the Coq code along with the
+tutorial. Use Ctrl+click to focus on a particular line.
 
 .. coq:: none
 |*)
@@ -164,7 +167,7 @@ Definition inverter_interface
      [mkPort "o" Bit]
      [].
 
-Compute (makeCircuitNetlist inverter_interface inverter).
+Compute makeCircuitNetlist inverter_interface inverter.
 
 (* A closer look at the circuit body *)
 Compute (makeCircuitNetlist inverter_interface inverter).(module).
@@ -180,15 +183,15 @@ Now, let's simulate the circuit, which can be useful for testing and proving
 functional correctness. Here, we use the identity-monad interpretation. The
 ``signal`` for this ``Cava`` instance is ``combType``, which interprets a
 ``Bit`` simply as a Coq ``bool``. If we provide the three inputs
-``[true; false; true]`` to the circuit simulation function ``multistep``, we'll
+``[true; false; true]`` to the circuit simulation function ``simulate``, we'll
 get ``[false; true; false]``:
 |*)
 
 (* identity-monad semantics *)
 Existing Instance CombinationalSemantics.
 
-Compute (simulate inverter [true; false; true]).
-Compute (simulate inverter [true; false; true; true; true; false]).
+Compute simulate inverter [true; false; true].
+Compute simulate inverter [true; false; true; true; true; false].
 
 (*|
 We can use the simulation to write proofs about the circuit. For instance, we
@@ -235,6 +238,11 @@ Proof.
 Qed.
 
 (*|
+A note about reading Coq proofs: in general, it's more important to understand
+the lemma statement (the part before ``Proof``) than it is to understand the
+proof body. The lemma statement shows what is being proven, and the proof body
+contains an "argument" to Coq that the statement is true.
+
 To summarize, there are three things you can do with Cava circuits:
 
 1. Define them (parameterized over an abstract ``Cava`` instance)
@@ -244,10 +252,354 @@ To summarize, there are three things you can do with Cava circuits:
 3. Simulate them using ``simulate``, and prove things about the simulations, by
    plugging in the ``CombinationalSemantics`` instance.
 
-In the next example, we'll try a slightly more complex circuit.
+In the following examples, we'll use this exact same three-part pattern to
+explore more complex circuits.
 
-Example 2 : 8-Bit xor
-=====================
+.. coq:: none
+|*)
+
+Section WithCava.
+  Context {signal} {semantics : Cava signal}.
+
+(*|
+Example 2 : Byte xor
+====================
+
+Our next example is a circuit that xors two bytes:
+|*)
+
+  Definition xor_byte :
+    Circuit (signal (Vec Bit 8) * signal (Vec Bit 8))
+            (signal (Vec Bit 8)) :=
+    Comb (fun '(v1, v2) => Vec.map2 xor2 v1 v2).
+
+(*|
+This circuit maps a 1-bit xor (``xor2``) over the two input vectors. ``xor2`` is
+one of the primitives provided by the ``Cava`` instance, like ``inv``. Once
+again, this is a combinational circuit, so we define it by wrapping a monadic
+function with ``Comb``.
+
+The ``Vec`` here is another ``SignalType``, with a slightly more complicated
+construction than ``Bit``. A ``Vec Bit 8`` is a vector of 8 bits: a
+byte. Vectors can be formed from any other ``SignalType``, including other
+vectors; ``Vec (Vec (Vec Bit 8) 4) 2)`` is a valid construction representing a
+two-dimensional array of bytes (equivalently, a three-dimensional array of
+bits).
+
+.. coq:: none
+|*)
+
+End WithCava.
+
+Local Open Scope vector_scope.
+
+(*|
+To generate a netlist for this circuit, we use mostly the same procedure as for
+the inverter, except that we change the input and output port types to match the
+circuit's type signature.
+|*)
+
+Definition xor_byte_interface
+  := sequentialInterface "xor_byte_interface"
+     "clk" PositiveEdge "rst" PositiveEdge
+     [mkPort "v1" (Vec Bit 8); mkPort "v2" (Vec Bit 8)]
+     [mkPort "o" (Vec Bit 8)]
+     [].
+
+Compute (makeCircuitNetlist xor_byte_interface xor_byte).(module).
+
+(*|
+Tuples in the input or output types become lists of ports for the netlist
+interface, so ``signal (Vec Bit 8) * signal (Vec Bit 8)`` becomes ``[mkPort "v1"
+(Vec Bit 8); mkPort "v2" (Vec Bit 8)]``. The names of the ports ("v1", "v2", and
+"o") are just for readability and potentially for reference by other netlists;
+they can be named however you prefer.
+
+We can also, as before, simulate the circuit.
+|*)
+
+Compute
+  simulate xor_byte
+  [([true;  true; true;  false; false; false; false; false],
+    [false; true; false; true;  false; false; false; false])].
+
+(*|
+Literal bit vectors are not especially readable, though; it's not immediately
+clear that this simulation is 7 xor 10 = 13. For simulations with bitvectors,
+it's often clearer to use natural-number-to-bitvector conversions from the Coq
+standard library :
+|*)
+
+Compute map Bv2N
+        (simulate xor_byte [(N2Bv_sized 8 7, N2Bv_sized 8 10)]).
+
+(*|
+Finally, we can prove that the circuit is correct. In this case, we prove that
+the circuit's behavior matches the ``BVxor`` definition from the standard
+library, specialized to bit-vectors of length 8.
+|*)
+
+Lemma xor_byte_correct (i : list (Vector.t bool 8 * Vector.t bool 8)) :
+  simulate xor_byte i = map (fun '(v1,v2) => BVxor 8 v1 v2) i.
+Proof.
+  cbv [xor_byte]. autorewrite with push_simulate.
+  apply map_ext; intros. destruct_pair_let.
+  cbv [BVxor]. simpl_ident.
+  apply Vector.map2_ext. reflexivity.
+Qed.
+
+(*|
+Again, no need to focus too much on the body of the proof here; understanding
+the lemma statement is the most important part. However, one interesting thing
+to note is that the proof is not computational; we don't analyze the 2^16
+possibile inputs separately. In fact, we never destruct the vectors or refer to
+the length at all, which leads us to our next example.
+
+Example 3: Bit-vector xor
+=========================
+
+As it turns out, we can define ``xor_byte`` over *arbitrary-length* bitvectors
+with very little modification. The circuit is virtually identical, except that
+it takes a length argument ``n`` and all the ``8``\ s are replaced with ``n``:
+
+.. coq:: none
+|*)
+
+Section WithCava.
+  Context {signal} {semantics : Cava signal}.
+
+(*||*)
+
+  Definition xor_bitvec (n : nat) :
+    Circuit (signal (Vec Bit n) * signal (Vec Bit n))
+            (signal (Vec Bit n)) :=
+    Comb (fun '(v1, v2) => Vec.map2 xor2 v1 v2).
+
+(*|
+.. coq:: none
+|*)
+
+End WithCava.
+
+(*|
+We can define an interface for this circuit that also takes ``n`` as an
+argument, and then compute a netlist for any number of gates we want.
+|*)
+
+Definition xor_bitvec_interface {n : nat}
+  := sequentialInterface "xor_bitvec_interface"
+     "clk" PositiveEdge "rst" PositiveEdge
+     [mkPort "v1" (Vec Bit n); mkPort "v2" (Vec Bit n)]
+     [mkPort "o" (Vec Bit n)]
+     [].
+
+(* Netlist for a 2-bit xor *)
+Compute
+  (makeCircuitNetlist xor_bitvec_interface (xor_bitvec 2)).(module).
+
+(* Netlist for a 100-bit xor! *)
+Compute
+  (makeCircuitNetlist xor_bitvec_interface (xor_bitvec 100)).(module).
+
+(*|
+Simulations are the same; just plug in any size.
+|*)
+
+(* 7 xor 10 = 13 (n=8) (same as xor_byte) *)
+Compute map Bv2N
+        (simulate (xor_bitvec 8) [(N2Bv_sized 8 7, N2Bv_sized 8 10)]).
+
+(* 1 xor 3 = 2 (n=2) *)
+Compute map Bv2N
+        (simulate (xor_bitvec 2) [(N2Bv_sized 2 1, N2Bv_sized 2 3)]).
+
+(* 1000 xor 3 = 1003 (n=10) *)
+Compute map Bv2N
+        (simulate (xor_bitvec 10)
+                  [(N2Bv_sized 10 1000, N2Bv_sized 10 3)]).
+
+(*|
+The correctness proof has is exactly the same as the ``xor_byte`` proof, except
+with ``n`` instead of ``8``; the proof body is completely unchanged.
+|*)
+
+Lemma xor_bitvec_correct
+      n (i : list (Vector.t bool n * Vector.t bool n)) :
+  simulate (xor_bitvec n) i = map (fun '(v1,v2) => BVxor n v1 v2) i.
+Proof.
+  cbv [xor_bitvec]. autorewrite with push_simulate.
+  apply map_ext; intros. destruct_pair_let.
+  cbv [BVxor]. simpl_ident.
+  apply Vector.map2_ext. reflexivity.
+Qed.
+
+(*|
+We can also easily prove that, for 8-bit vectors, ``xor_bitvec`` is equivalent
+to ``xor_byte``:
+|*)
+
+Lemma xor_bitvec_xor_byte_equiv
+      (i : list (Vector.t bool 8 * Vector.t bool 8)) :
+  simulate (xor_bitvec 8) i = simulate xor_byte i.
+Proof. reflexivity. Qed.
+
+(*|
+This example demonstrates the advantage of using a proof assistant instead of a
+more computational method. The ``xor_bitvec_correct`` proof checks essentially
+instantly and holds for *all* values of ``n``. With one circuit definition, and
+one proof, you have defined every single length of bit-vector xor you'll ever
+need. The same principle can apply to more complicated structures as well.
+
+Example 4: Tree of xors
+=======================
+
+.. coq:: none
+|*)
+
+Section WithCava.
+  Context {signal} {semantics : Cava signal}.
+
+(*|
+To take the last circuit a step further, let's consider xoring not just two
+``n``-length vectors, but an arbitrary number ``m`` of ``n``-length vectors!
+
+We could write a definition that chains the xors together one by one::
+
+  xor (xor (xor (xor (xor a b) c) d) e f)
+
+
+However, since there are no data dependencies, the circuit will have better
+timing properties for possibly large ``m`` if it is a tree, e.g.::
+
+  xor (xor (xor a b) c) (xor (xor d e) f)
+
+Luckily, Cava's standard library (which you can import with ``Require Import
+Cava.Cava``) contains a ``tree`` combinator for exactly this kind of situation.
+|*)
+
+  Definition xor_tree {n m : nat} :
+    Circuit (signal (Vec (Vec Bit n) m))
+            (signal (Vec Bit n)) :=
+    Comb (tree (fun '(v1, v2) => Vec.map2 xor2 v1 v2)).
+
+(*|
+.. coq:: none
+|*)
+
+End WithCava.
+
+(*|
+Now, we can just plug in any sequence of same-size vectors and compute the
+results!
+|*)
+
+(* 7 xor 10 = 13 (n=8, m=2)*)
+Compute map Bv2N
+        (simulate xor_tree
+                  [[N2Bv_sized 8 7; N2Bv_sized 8 10]]).
+
+(* 1000 xor 3 = 1003 (n=10, m=2) *)
+Compute map Bv2N
+        (simulate (xor_bitvec 10)
+                  [(N2Bv_sized 10 1000, N2Bv_sized 10 3)]).
+
+(* 1 xor 2 xor 4 xor 8 xor 16 xor 32 xor 64 xor 128 = 255 (n=8, m=8) *)
+Compute map Bv2N
+        (simulate xor_tree
+                  [[ N2Bv_sized 8 1
+                     ; N2Bv_sized 8 2
+                     ; N2Bv_sized 8 4
+                     ; N2Bv_sized 8 8
+                     ; N2Bv_sized 8 16
+                     ; N2Bv_sized 8 32
+                     ; N2Bv_sized 8 64
+                     ; N2Bv_sized 8 128
+                   ]]).
+
+(*|
+To prove the xor tree circuit correct, we prove that it's equivalent to a
+``fold_left``, which is a native Coq loop. Essentially, this proof says that the
+circuit, even with the tree structure, is equivalent to just chaining ``BVxor``
+over the input in order (starting with 0, which is the identity for xor).
+
+.. coq:: none
+|*)
+
+Hint Rewrite Nxor_BVxor using solve [eauto] : push_Bv2N.
+
+(*||*)
+
+Lemma xor_tree_correct n m (i : list (Vector.t (Vector.t bool n) m)) :
+  m <> 0 -> (* rule out size-0 tree *)
+  simulate xor_tree i = map (fun vs =>
+                               Vector.fold_left
+                                 (BVxor n) (N2Bv_sized n 0) vs) i.
+Proof.
+  cbv [xor_tree]. intros.
+  autorewrite with push_simulate.
+  apply map_ext; intros.
+
+  (* this rewrite produces side conditions; we'll handle them later *)
+  rewrite @tree_equiv with (t:=Vec Bit n) (id:=N2Bv_sized n 0);
+    intros; auto; simpl_ident.
+
+  { (* xor circuit is equivalent to BVxor *)
+    cbv [BVxor].
+    apply Vector.fold_left_ext; intros; simpl_ident.
+    apply Vector.map2_ext. reflexivity. }
+
+  (* now, solve the tree_equiv side conditions *)
+
+  { (* 0 is a left identity *)
+    apply Bv2N_inj. autorewrite with push_Bv2N.
+    apply N.lxor_0_l. }
+  { (* 0 is a right identity *)
+    apply Bv2N_inj. autorewrite with push_Bv2N.
+    apply N.lxor_0_r. }
+  { (* xor is associative *)
+    apply Bv2N_inj. autorewrite with push_Bv2N.
+    symmetry. apply N.lxor_assoc. }
+Qed.
+
+(*|
+It's worth taking a moment here again to point out just how broad the proof of
+correctness is. This proof applies to a circuit that xors two bits, and also
+applies to a circuit that xors 1000 1000-bit bitvectors.
+
+As a final touch, we can also prove that, when applied to just two bitvectors
+(``m = 2``), ``xor_tree`` is equivalent to ``xor_bitvec``:
+|*)
+
+Lemma xor_bitvec_xor_tree_equiv
+      n (i : list (Vector.t bool n * Vector.t bool n)) :
+  simulate (xor_bitvec n) i =
+  simulate xor_tree (map (fun '(v1,v2) => [v1;v2]) i).
+Proof.
+  cbv [xor_bitvec xor_tree]; autorewrite with push_simulate.
+  rewrite map_map.
+  apply map_ext; intros. destruct_pair_let.
+
+  (* The tree lemma produces the same side conditions as before, but
+     we solve them here in a more concise way *)
+  erewrite @tree_equiv with
+      (t:=Vec Bit n) (id:=N2Bv_sized n 0)
+    by (intros; auto; simpl_ident; apply Bv2N_inj;
+        autorewrite with push_Bv2N;
+        auto using N.lxor_0_r, N.lxor_0_l, N.lxor_assoc).
+
+  autorewrite with push_vector_fold vsimpl. simpl_ident.
+  apply Bv2N_inj. autorewrite with push_Bv2N.
+  rewrite N.lxor_0_l. reflexivity.
+Qed.
+
+(*|
+At this point, we've covered pretty much everything you need to start building
+*combinational* circuits in Cava -- circuits that don't have any
+timing-dependent elements like loops or registers. In the next example, we'll
+show how to build *sequential* circuits.
+
+Example 5 : Counter
+===================
 
 To be continued!
 |*)
